src/Util/FisherYates/Model.dfy
@@ -12,20 +12,41 @@ module FisherYates.Model {
    Definitions
   ************/
 
+  ghost predicate ShuffleInvariancePredicatePointwise<T>(xs: seq<T>, r: Monad.Result<seq<T>>, j: int)
+    requires 0 <= j < |xs|
+  {
+    r.Result? ==> |r.value| == |xs| && r.value[j] == xs[j]
+  }
+
   ghost function Shuffle<T>(xs: seq<T>, i: nat := 0): (h: Monad.Hurd<seq<T>>)
     requires i <= |xs|
-    decreases |xs| - i
     ensures forall s :: h(s).Result? ==> multiset(h(s).value) == multiset(xs) && |h(s).value| == |xs|
-    ensures forall s, j | 0 <= j < i :: h(s).Result? ==> h(s).value[j] == xs[j]
+    ensures forall s, j | 0 <= j < i :: ShuffleInvariancePredicatePointwise(xs, h(s), j)
   {
-    (s: Rand.Bitstream) =>
-      if |xs[i..]| > 1 then
-        var (j, s') :- Uniform.Model.IntervalSample(i, |xs|)(s);
-        assert i <= j < |xs| by { Uniform.Model.IntervalSampleBound(i, |xs|, s); }
-        var ys := Swap(xs, i, j);
-        Shuffle(ys, i + 1)(s')
-      else
-        Monad.Return(xs)(s)
+    (s: Rand.Bitstream) => ShuffleCurried(xs, s, i)
+  }
+
+  ghost function ShuffleCurried<T>(xs: seq<T>, s: Rand.Bitstream, i: nat := 0): (r: Monad.Result<seq<T>>)
+    requires i <= |xs|
+    decreases |xs| - i
+    ensures r.Result? ==> multiset(r.value) == multiset(xs) && |r.value| == |xs|
+    ensures forall j | 0 <= j < i :: ShuffleInvariancePredicatePointwise(xs, r, j)
+  {
+    if |xs| - i > 1 then
+      var (j, s') :- Uniform.Model.IntervalSample(i, |xs|)(s);
+      assert i <= j < |xs| by { Uniform.Model.IntervalSampleBound(i, |xs|, s); }
+      var ys := Swap(xs, i, j);
+      var r := ShuffleCurried(ys, s', i + 1);
+      assert forall j | 0 <= j < i :: ShuffleInvariancePredicatePointwise(xs, r, j) by {
+        forall j | 0 <= j < i 
+          ensures ShuffleInvariancePredicatePointwise(xs, r, j) 
+        {
+          assert ShuffleInvariancePredicatePointwise(ys, r, j);
+        }
+      }
+      r
+    else
+      Monad.Return(xs)(s)
   }
 
   function Swap<T>(s: seq<T>, i: nat, j: nat): (t: seq<T>)
